add type env, add parser & pretty-printer

src/ocaml/parser/ast.ml
@@ -1,0 +1,346 @@
+(*open Set*)
+
+   
+let fgtyp_delim = "@"
+            
+(** Types *)
+
+type size = Z.t
+
+type fgtyp =
+  Tuint of size
+| Tsint of size
+
+let uint_t w = Tuint w
+let int_t w = Tsint w
+(*let bit_t = Tuint 1*)
+
+(*
+let z_two = Z.of_int 2
+
+let string_of_fgtyp ty =
+  match ty with
+  | Tuint w -> "uint" ^ string_of_int w
+  | Tsint w -> "int" ^ string_of_int w
+let size_of_fgtyp ty =
+  match ty with
+  | Tuint w -> w
+  | Tsint w -> w
+let min_of_fgtyp ty =
+  match ty with
+  | Tuint _w -> Z.zero
+  | Tsint w -> Z.neg (Z.pow z_two (w - 1))
+let max_of_fgtyp ty =
+  match ty with
+  | Tuint w -> Z.sub (Z.pow z_two w) Z.one
+  | Tsint w -> Z.sub (Z.pow z_two (w - 1)) Z.one
+let fgtyp_is_signed ty =
+  match ty with
+  | Tsint _ -> true
+  | Tuint _ -> false
+let fgtyp_to_signed ty =
+  match ty with
+  | Tuint w -> Tsint w
+  | Tsint _w -> ty
+let fgtyp_to_unsigned ty =
+  match ty with
+  | Tuint _w -> ty
+  | Tsint w -> Tuint w
+ *)
+            
+type var = string
+             
+(*
+(** Variables with SSA index taken into consideration *)
+
+type var =
+  {
+    vname : string;     (* name of the variable *)
+    vtyp : fgtyp;         (* type of the variable *)
+    vsidx : int         (* SSA index of the variable *)
+  }
+
+let invalid_sidx i = i < 0
+let default_non_ssa_idx = -1
+(*
+ * The string representation of a variable with SSA index taken into consideration
+ * If the argument labeled with vtyp is true, the variable type is also output.
+ *)
+let string_of_var ?fgtyp:(fgtyp=false) v =
+  let str =
+    if invalid_sidx v.vsidx then v.vname
+    else v.vname ^ "_" ^ string_of_int v.vsidx in
+  if fgtyp then str ^ fgtyp_delim ^ string_of_fgtyp v.vtyp
+  else str
+let size_of_var v = size_of_fgtyp v.vtyp
+let fgtyp_of_var v = v.vtyp
+(* Two variables are equal if
+ * - they have the same name and
+ * - their SSA indices are equal.
+ *)
+let eq_var v1 v2 = v1.vname = v2.vname && v1.vsidx = v2.vsidx
+let cmp_var v1 v2 =
+  let c = Pervasives.compare v1.vname v2.vname in
+  if c = 0 then Pervasives.compare v1.vsidx v2.vsidx
+  else c
+let mem_var v vs = List.exists (fun u -> eq_var u v) vs
+let mkvar vn vt = { vname = vn; vtyp = vt; vsidx = default_non_ssa_idx }
+let var_is_uint v =
+  match v.vtyp with
+  | Tuint _ -> true
+  | _ -> false
+let var_is_sint v =
+  match v.vtyp with
+  | Tsint _ -> true
+  | _ -> false
+let var_is_bit v = v.vtyp = bit_t
+let var_is_signed v = fgtyp_is_signed v.vtyp
+
+module VarElem : OrderedType with type t = var =
+  struct
+    type t = var
+    let compare = cmp_var
+  end
+module VS = Set.Make(VarElem)
+module VM = Map.Make(VarElem)
+
+
+let vs_disjoint vs1 vs2 = VS.is_empty (VS.inter vs1 vs2)
+let string_of_vs ?fgtyp:(fgtyp=false) vs = String.concat ", " (List.map (fun v -> string_of_var ~fgtyp:fgtyp v) (VS.elements vs))
+
+(** Syntax *)
+
+type numeral = Z.t
+
+type decimal = string
+
+(* A hexadecimal number is a string with MSB at the beginning *)
+type hex = string
+
+(* A binary number is a string of 0's and 1's with MSB at the head *)
+type binary = string
+
+type symbol = string
+            
+(* type spec_constant =
+ *   | CNumeral of numeral
+ *   | CDecimal of decimal
+ *   | CHexDecimal of hex
+ *   | CBinary of binary
+ *   | CString of string
+ * 
+ * (\* A keyword always starts with a ":" *\)
+ * type keyword = string
+ * 
+ * type attribute =
+ *   | AKeyword of keyword
+ *   | AConstant of keyword * spec_constant
+ *   | ASymbol of keyword * symbol
+ * 
+ * type solver_option =
+ *   | OKeyword of keyword
+ *   | OConstant of keyword * spec_constant
+ *   | OSymbol of keyword * symbol
+ *              
+ * type index =
+ *   | INumeral of numeral
+ *   | ISymbol of symbol
+ * 
+ * type identifier =
+ *   | ISimple of symbol                             (\* Simple Identifier *\)
+ *   | IIndexed of symbol * index list               (\* Indexed Identifier *\)
+ * 
+ * type sort =
+ *   | SIdentifier of identifier
+ *   | SApplication of identifier * sort list
+ * 
+ * type qual_identifier =
+ *   | QIdentifier of identifier
+ *   | QAnnotated of identifier * sort
+ * 
+ * type var_binding = symbol * term
+ * 
+ * and term =
+ *   | TConstant of spec_constant
+ *   | TVariable of qual_identifier
+ *   | TApplication of qual_identifier * term list
+ *   | TLet of var_binding list * term
+ * 
+ * type sorted_var = symbol * sort
+ * 
+ * type command =
+ *   | CSetLogic of symbol
+ *   | CSetInfo of attribute
+ *   | CSetOption of solver_option
+ *   | CDeclareFun of symbol * sort list * sort
+ *   | CDefineFun of symbol * sorted_var list * sort * term
+ *   | CAssert of term
+ *   | CCheckSat
+ *   | CGetModel
+ *   | CExit
+ *   | CComment of string *)
+ *)
+             
+(** Operators *)
+
+type ucast =
+  | AsUint | AsSInt | AsFixed | AsClock
+              
+type eunop =
+  | Upadding of Z.t
+  | Ucast of ucast
+  | Ushl of Z.t
+  | Ushr of Z.t
+  | Ucvt
+  | Uneg
+  | Unot
+  | Uandr
+  | Uorr
+  | Uxorr
+  | Uextr of Z.t * Z.t
+  | Uhead of Z.t
+  | Utail of Z.t
+  | Uincp
+  | Udecp
+  | Usetp
+              
+type bcmp =
+  | Blt | Bleq | Bgt | Bgeq | Beq | Bneq
+
+type ebinop =
+  | Badd
+  | Bsub
+  | Bmul
+  | Bdiv
+  | Brem
+  | Bcomp of bcmp
+  | Bdshl
+  | Bdshr
+  | Band
+  | Bor
+  | Bxor
+  | Bcat
+
+type fexpr =
+  | Econst of int
+  | Evar of var
+  | Eref of var * fgtyp
+  | Efield of var * fexpr
+  | Esubacc of var * Z.t
+  | Eprim_unop of eunop * fexpr
+  | Eprim_binop of ebinop * fexpr * fexpr
+  | Emux of fexpr * fexpr * fexpr
+  | Evalidif of fexpr
+                                   
+type ruw =
+  | RUWold | RUWnew | RUWundefined
+
+
+type fmem =
+  {
+    mid : var;
+    data_type : fexpr;
+    depth : Z.t;
+    reader : var list;
+    writer : var list;                    
+    read_latency : Z.t;
+    write_latency : Z.t;
+    read_write : ruw
+  }
+
+type freg =
+  {
+    rid : var;
+    rtype : fexpr;
+    reset : fexpr list
+  }
+
+type fstmt =
+  | Sskip
+  | Swire of var * fgtyp
+  | Sreg of freg
+  | Smem of fmem
+  | Sinst of var * var
+  | Snode of var * fexpr
+  | Sfcnct of fexpr * fexpr
+  | Spcnct of fexpr * fexpr
+  | Sinvalid of var
+  | Sattach of var list
+  | Swhen of fexpr * fstmt * fstmt
+  | Sstop of fexpr * fexpr * Z.t
+  | Sprintf (* TBD *)
+  | Sassert (* TBD *)
+  | Sassume (* TBD *)
+  | Sdefname of var (* TBD *)
+  | Sparam of var * fexpr (* TBD *)
+
+type fport =
+  | Finput of fexpr
+  | Foutput of fexpr
+
+type fmodule =
+  | FInmod of var * fport list * fstmt list
+  | FExmod of var * fport list * fstmt list
+
+type fcircuit = var * fmodule list
+                  
+type file = fcircuit
+
+
+let pp_type out ty =
+  match ty with
+  | Tuint s -> output_string out "(Tunit "; output_string out (Z.to_string s); output_string out ")"
+  | Tsint s -> output_string out "(Tsnit "; output_string out (Z.to_string s); output_string out ")"
+          
+let pp_unop out op =
+  match op with
+  | Unot -> output_string out "Unot ";
+  | _ -> output_string out ""
+       
+let pp_binop out op =
+  match op with
+  | Badd -> output_string out "Badd ";
+  | _ -> output_string out ""
+          
+let rec pp_expr out e =
+  match e with
+  | Evar v -> output_string out "(Evar "; output_string out (v^" "); output_string out ")"
+  | Eref (v, ty) -> output_string out "(Eref "; output_string out (v^" "); output_string out " "; pp_type out ty; output_string out ")\n"
+  | Eprim_unop (op, e1) -> output_string out "(Eprim_unop "; pp_unop out op; pp_expr out e1; output_string out ")"
+  | Eprim_binop (bop, e1, e2) -> output_string out "(Eprim_binop "; pp_binop out bop; pp_expr out e1; output_string out " "; pp_expr out e2; output_string out ")"
+  | _ -> output_string out ""
+
+let pp_exprs out el =  List.iter (fun c -> pp_expr out c; output_string out "") el
+
+let rec pp_ports out pl =  List.iter (fun c -> pp_port out c; output_string out "") pl
+                     
+and pp_port out p =
+  match p with
+  | Finput e -> output_string out "(Finput "; pp_expr out e; output_string out ")\n"
+  | Foutput e -> output_string out "(Foutput "; pp_expr out e; output_string out ")\n"                 
+                 
+
+let rec pp_statements out sl = List.iter (fun c -> pp_statement out c; output_string out "") sl
+                             
+and  pp_statement out s =
+  match s with
+  | Sskip -> output_string out "(Sskip)"
+  | Swire (v, ty) -> output_string out "(Swire "; output_string out (v^" "); pp_type out ty; output_string out ")\n"
+  | Sfcnct (e1, e2) -> output_string out "(Sfcnct "; pp_expr out e1; output_string out " "; pp_expr out e2; output_string out ")\n"
+  | Spcnct (e1, e2) -> output_string out "(Spcnct "; pp_expr out e1; output_string out " "; pp_expr out e2; output_string out ")\n"
+  | Swhen (e, s1, s2) -> output_string out "(Swhen "; pp_expr out e; pp_statement out s1; pp_statement out s2; output_string out ")\n"
+  | _ -> output_string out ""
+                 
+          
+let pp_module out fmod =
+  match fmod with
+  | FInmod (v, pl, sl) -> output_string out "(FInmod "; output_string out (v^" "); pp_ports out pl; pp_statements out sl; output_string out ")\n"
+  | _ -> output_string out "\n"
+          
+let pp_modules out fmod = List.iter (fun c -> pp_module out c; output_string out "") fmod
+
+let pp_fcircuit out fc =
+  match fc with
+  | (v, fmod) -> output_string out "(FCircuit "; output_string out (v^" "); pp_modules out fmod; output_string out ")"
+
+let pp_file out fc = pp_fcircuit out fc
