src/ocaml/parser/firrtlLexer.mll
@@ -1,0 +1,74 @@
+{
+  open FirrtlParser
+
+  exception Error of string
+  let lnum = ref 1
+  let cnum = ref 0
+  let get_len lexbuf = String.length (Lexing.lexeme lexbuf)
+  let upd_cnum lexbuf = cnum := !cnum + get_len lexbuf
+  let reset_cnum () = cnum := 0
+}
+
+let digit = ['0'-'9']
+let binary_digit = ['0' '1']
+let numeral = '0' | ['1'-'9'] digit*
+let letter = ['a'-'z' 'A'-'Z' '_']
+let special_char = ['+' '-' '/' '*' '=' '%' '?' '!' '.' '$' '_' '~' '&' '^' '<' '>' '@' '\'']
+let symbol = ('|' [^'|']+ '|') | (letter|special_char)(letter|special_char|digit)*
+let escape_space = "\"\""
+
+let letter = ['a'-'z' 'A'-'Z' '_']
+let number = ['0'-'9']
+let hex = ['0'-'9' 'a'-'f' 'A'-'F']
+let identity = letter (letter | number)*
+let comment_line = ("//"([^ '\n' ]+))|('#'([^ '\n' ]+))
+
+rule token = parse
+| [' ' '\t']                            { upd_cnum lexbuf; token lexbuf }
+| ("\r\n"|'\n'|'\r')                    { reset_cnum(); incr lnum; token lexbuf }
+| '('                                   { upd_cnum lexbuf; PAR_OPEN }
+| ')'                                   { upd_cnum lexbuf; PAR_CLOSE }
+| '<'                                   { upd_cnum lexbuf; ANG_OPEN }
+| '>'                                   { upd_cnum lexbuf; ANG_CLOSE }
+| '['                                   { upd_cnum lexbuf; SQR_OPEN }
+| ']'                                   { upd_cnum lexbuf; SQR_CLOSE }
+| '"'                                   { upd_cnum lexbuf; QUOT }
+| '_'                                   { upd_cnum lexbuf; UNDERSCORE }
+| "b" (binary_digit+ as str)            { upd_cnum lexbuf; BINARY str }
+| "o" (numeral+ as str)                 { upd_cnum lexbuf; OCTAL str }
+| ':'                                   { upd_cnum lexbuf; KEYWORD }
+| ','                                   { upd_cnum lexbuf; SPRT }
+| '.'                                   { upd_cnum lexbuf; SUB_FIELD }
+| "h" (hex+ as str)
+                                        { upd_cnum lexbuf; HEX_DECIMAL str }
+| numeral '.' '0'* numeral as str       { upd_cnum lexbuf; DECIMAL str }
+| numeral as str                        { upd_cnum lexbuf; NUMERAL str }
+| '"' (([^'"']|escape_space)* as str) '"'
+                                        { upd_cnum lexbuf; STRING str }
+| "circuit"                             { upd_cnum lexbuf; CIRCUIT }
+| "module"                              { upd_cnum lexbuf; STM_MODULE }
+| "skip"                                { upd_cnum lexbuf; STM_SKIP }
+| "input"                               { upd_cnum lexbuf; STM_INPUT }
+| "output"                              { upd_cnum lexbuf; STM_OUTPUT }
+| "when"                                { upd_cnum lexbuf; STM_WHEN }
+| "else"                                { upd_cnum lexbuf; STM_ELSE }
+| "<="                                  { upd_cnum lexbuf; STM_CONNECT }
+| "<-"                                  { upd_cnum lexbuf; STM_PCONNECT}
+| "add"                                 { upd_cnum lexbuf; EXPR_ADD}
+| "not"                                 { upd_cnum lexbuf; EXPR_NOT}
+| "wire"                                { upd_cnum lexbuf; STM_WIRE }
+(*
+| "reg"                                 { upd_cnum lexbuf; STM_REG }
+| "mem"                                 { upd_cnum lexbuf; STM_MEM }
+ *)
+(* Types *)
+| "UInt"                                { upd_cnum lexbuf; UINT }
+| "SInt"                                { upd_cnum lexbuf; SINT }
+| "Int"                                 { upd_cnum lexbuf; SINT }
+(*
+| "Analog"                       { upd_cnum lexbuf; ANALOG }
+| "Clock"                        { upd_cnum lexbuf; CLOCK }
+| "Fixed"                        { upd_cnum lexbuf; FIXED }
+ *)
+| symbol as str                         { upd_cnum lexbuf; SYMBOL str }
+| eof                            { EOF }
