src/ocaml/parser/firrtlParser.mly
@@ -1,0 +1,117 @@
+%{
+    open Ast
+
+%}
+
+%token<string> COMMENT
+%token<string> BINARY HEX_DECIMAL OCTAL DECIMAL NUMERAL STRING SYMBOL
+%token PAR_OPEN PAR_CLOSE ANG_OPEN ANG_CLOSE SQR_OPEN SQR_CLOSE UNDERSCORE QUOT SPRT KEYWORD
+%token CIRCUIT STM_MODULE STM_SKIP STM_INPUT STM_OUTPUT STM_WHEN STM_ELSE  STM_CONNECT STM_PCONNECT
+%token STM_WIRE STM_REG STM_MEM EXPR_ADD EXPR_NOT SUB_FIELD UINT SINT INT
+%token EOF
+
+%start file
+%type <Ast.file> file
+
+%%
+
+file
+  : circuit EOF                          { $1 }
+;
+
+circuit
+  : cct fmodules                         { ($1, $2)}
+  ;
+
+cct
+  : CIRCUIT symbol KEYWORD               { $2 }
+  ;
+    
+fmodules
+  :                                      { [] }
+  | fmodule fmodules                     { $1::$2}
+  ;
+    
+fmodule
+  : mdl ports statements                 { FInmod ($1, $2, $3) }
+  ;
+
+mdl 
+  : STM_MODULE symbol KEYWORD            { $2 }
+  ;
+
+ports
+  :                                      { [] }
+  | port ports                           { $1::$2 }
+  ;    
+
+port
+  : STM_INPUT symbol KEYWORD typ_def
+                                         { Finput (Eref ($2, $4)) }
+  | STM_OUTPUT symbol KEYWORD typ_def
+                                         { Foutput (Eref ($2, $4)) }
+;
+
+typ_def
+  :  UINT ANG_OPEN numeral ANG_CLOSE      { Tuint $3 }
+  | SINT ANG_OPEN numeral ANG_CLOSE      { Tsint $3 }
+;
+
+/* statement */
+
+statements
+  :                                      { [] }
+  | statement statements                 { $1::$2 }
+  ;    
+
+statement
+  : STM_SKIP
+	                                    { Sskip }
+  | STM_WHEN expr KEYWORD statement STM_ELSE KEYWORD statement
+                                            { Swhen ($2, $4, $7) }
+  | expr STM_CONNECT expr
+                                            { Sfcnct ( $1, $3) }
+  | expr STM_PCONNECT expr
+                                            { Spcnct ( $1, $3) } 
+  | STM_WIRE symbol KEYWORD typ_def 
+                                            { Swire ($2, $4) } 
+;
+  
+/* expression */
+  
+expr
+:   symbol                                  { Evar $1 }
+  | EXPR_ADD PAR_OPEN symbol SPRT symbol PAR_CLOSE
+                                            { Eprim_binop (Badd, (Evar $3), (Evar $5))}
+  | EXPR_NOT PAR_OPEN symbol PAR_CLOSE
+                                            { Eprim_unop (Unot, (Evar $3))}
+;  
+
+/* Symbols */
+
+symbol
+  : SYMBOL                              { $1 }
+;
+
+
+/* spec_constant */
+
+numeral
+  : NUMERAL                             { Z.of_string $1 }
+;
+
+decimal
+  : DECIMAL                             { $1 }
+;
+
+hexadecimal
+  : HEX_DECIMAL                         { String.uppercase_ascii $1 }
+;
+
+binary
+  : BINARY                              { $1 }
+;
+
+string
+  : STRING                              { $1 }
+;
