src/ocaml/parser/parser.ml
@@ -1,0 +1,5 @@
+open FirrtlParser
+
+let parse file =
+  let lexbuf = Lexing.from_channel (open_in file) in
+  FirrtlParser.file FirrtlLexer.token lexbuf
