src/ocaml/pparser.ml
@@ -1,0 +1,19 @@
+
+open Firrtl_lang
+
+  
+let output_file = ref None
+let file = "./demo/demo"
+                
+let pparse file =
+  let f = (Parser.parse file) in
+  let out =
+    match !output_file with
+    | None -> stdout
+    | Some fn -> open_out fn in
+  let _ = Ast.pp_file out f in
+  let _ = flush out in
+  close_out out
+
+
+let _ =  pparse file
