src/Firrtl.v
@@ -1,179 +1,376 @@
-From Coq Require Import ZArith Arith RelationClasses OrderedType.
-From mathcomp Require Import ssreflect ssrbool ssrnat eqtype seq.
+(*From Coq Require Import ZArith Arith RelationClasses OrderedType FMaps FSets FunInd FMapAVL.*)
 
-(****** Types ******)
+From Coq Require Import FunInd FMaps FMapAVL OrderedType.
+From mathcomp Require Import ssreflect ssrbool ssrnat ssrint eqtype seq.
+From simplssrlib Require Import Types Tactics .
 
-(****** Ground Types ******)
+Set Implicit Arguments.
+Unset Strict Implicit.
+Import Prenex Implicits.
 
-Inductive fgtyp : Set :=
-  Fuint : nat -> fgtyp
-| Fsint : nat -> fgtyp
-| Fanalog : nat -> fgtyp
-| Fclock
-| Ffixed : nat -> Z -> fgtyp
-| Fvector : fgtyp -> fgtyp -> fgtyp.
+Section RawFirrtl.
+  (****** Types Environment ******)
 
+  (****** Ground Types ******)
 
-(* Integer, bitvector or ssrint, TBD *)
-Definition fbits := Type.
+  From Coq Require Import ZArith.
 
-Inductive fint : Type :=
-| UInt : fbits -> fint
-| SInt : fbits -> fint.
+  Inductive fgtyp : Set :=
+    Fuint : nat -> fgtyp
+  | Fsint : nat -> fgtyp
+  | Fanalog : nat -> fgtyp
+  | Fclock
+  | Ffixed : nat -> Z -> fgtyp.
+  (*| Fvector : fgtyp -> nat -> fgtyp.*)
 
-(* Fix-point, TBD *)
+  (* Size of types *)
 
-(* Analog, TBD *)
+  Definition sizeof_fgtyp (t : fgtyp) : nat :=
+    match t with
+    | Fuint w => w
+    | Fsint w => w
+    | Fanalog w => w
+    | Fclock => 1
+    | Ffixed n z => n
+    end.
 
-(* Vector, TBD *)
+  (* Equality of types *)
 
-(*
-(****** Type Equivalence ******)
+  Lemma fgtyp_eq_dec (x y : fgtyp) : {x = y} + {x <> y}.
+  Proof.
+    destruct x; destruct y; try (intros; right; move=> []; discriminate).
+    - intros; case: (Nat.eq_dec n n0) => H.
+      + left; rewrite H; reflexivity.
+      + right; move=> []; auto.
+    - intros; case: (Nat.eq_dec n n0) => H.
+      + left; rewrite H; reflexivity.
+      + right; move=> []; auto.
+    - intros; case: (Nat.eq_dec n n0) => H.
+      + left; rewrite H; reflexivity.
+      + right; move=> []; auto.
+    - left; done.
+    - intros; case: (Nat.eq_dec n n0) => H;
+                                           case: (Z.eq_dec z z0) => H0.
+      + left; rewrite H H0; reflexivity.
+      + right; move=> []; auto.
+      + right; move=> []; auto. 
+      + right; move=> []; auto.
+  Qed.
 
-(* TBD *)
-Parameter fint_to_Z : fbits -> Z.
+  Definition fgtyp_eqn (x y : fgtyp) : bool :=
+    match x, y with
+    | Fuint wx, Fuint wy => wx == wy
+    | Fsint wx, Fsint wy => wx == wy
+    | Fanalog wx, Fanalog wy => wx == wy
+    | Fclock, Fclock => true
+    | Ffixed wx bpx, Ffixed wy bpy => (wx == wy) && (Zeq_bool bpx bpy)
+    | _, _ => false
+    end.
 
-(* Integer type eq *)
+  Notation "x =? y" := (fgtyp_eqn x y).
 
-Definition fint_eq fi1 fi2 :=
-  match fi1, fi2 with
-  | UInt bs1, UInt bs2 => Zeq_bool (fint_to_Z bs1) (fint_to_Z bs2)
-  | SInt bs1, SInt bs2 => Zeq_bool (fint_to_Z bs1) (fint_to_Z bs2)
-  | UInt _, SInt _ => false
-  | SInt _, UInt _ => false
-  end.
-*)
-                        
-(****** Syntax ******)
+  Lemma fgtyp_eqn_refl (x : fgtyp) : x =? x.
+  Proof.
+    destruct x; try (exact: eqxx).
+    - done.
+    - rewrite/=; rewrite eqxx andTb. by apply Zeq_is_eq_bool.
+  Qed.
 
-(****** Expressions ******)
+  Lemma fgtyp_eqn_eq (x y : fgtyp) : x =? y <-> x = y.
+  Proof.
+    split; first (destruct x; destruct y; move=> /= H);
+      try (discriminate|| rewrite (eqP H); reflexivity).
+    - done.
+    - move/andP : H => [H1 H2]; by rewrite (eqP H1) (Zeq_bool_eq _ _ H2).
+    - move=> ->. exact: fgtyp_eqn_refl.
+  Qed.
 
-(* Import ssrlib, TBD *)
-Variable var : eqType.
+  Lemma fgtyp_eqn_sym (x y : fgtyp) : x =? y -> y =? x.
+  Proof.
+    move/fgtyp_eqn_eq => H. apply/fgtyp_eqn_eq. symmetry. assumption.
+  Qed.
 
-Inductive ucast : Set :=
-| AsUInt | AsSInt | AsFixed | AsClock.
+  Lemma fgtyp_eqn_trans (x y z : fgtyp) : x =? y -> y =? z -> x =? z.
+  Proof.
+    move/fgtyp_eqn_eq => Hxy. move/fgtyp_eqn_eq => Hyz. apply/fgtyp_eqn_eq.
+    rewrite Hxy. assumption.
+  Qed.
 
-Inductive eunop : Set :=
-| Upadding : nat -> eunop
-| Ucast : ucast -> eunop
-| Ushl : nat -> eunop
-| Ushr : nat -> eunop
-| Ucvt
-| Uneg
-| Unot
-| Uandr
-| Uorr
-| Uxorr
-| Uextr : nat -> nat -> eunop
-| Uhead : nat -> eunop
-| Utail : nat -> eunop
-| Uincp
-| Udecp
-| Usetp .
+  Instance fgtyp_eqn_Reflexive : Reflexive (@fgtyp_eqn) := @fgtyp_eqn_refl.
+  Instance fgtyp_eqn_Symmetric : Symmetric (@fgtyp_eqn) := @fgtyp_eqn_sym.
+  Instance fgtyp_eqn_Transitive : Transitive (@fgtyp_eqn) := @fgtyp_eqn_trans.
+  Instance fgtyp_eqn_Equivalence : Equivalence (@fgtyp_eqn) :=
+    { Equivalence_Reflexive := fgtyp_eqn_Reflexive;
+      Equivalence_Symmetric := fgtyp_eqn_Symmetric;
+      Equivalence_Transitive := fgtyp_eqn_Transitive }.
 
-Inductive bcmp : Set :=
-| Blt | Bleq | Bgt | Bgeq | eq | neq.
+  Lemma fgtyp_eqP : forall (x y : fgtyp), reflect (x = y) (x =? y).
+  Proof.
+    move=> x y. case H: (x =? y).
+    - apply: ReflectT. apply/fgtyp_eqn_eq. assumption.
+    - apply: ReflectF. move=> Heq. move/fgtyp_eqn_eq: Heq => Heq. rewrite Heq in H.
+      discriminate.
+  Qed.
 
-Inductive ebinop : Set :=
-| Badd
-| Bsub
-| Bmul
-| Bdiv
-| Brem
-| Bcomp: bcmp -> ebinop
-| Bdshl
-| Bdshr
-| Band
-| Bor
-| Bxor
-| Bcat .
-
-(* mux, valid, sub-xxx, TBD *)
-Inductive fexpr : Type :=
-| Econst : fint -> fexpr
-| Eref : var -> fgtyp -> fexpr
-| Efield : var -> fexpr -> fexpr
-| Esubacc : var -> nat -> fexpr
-| Eprim_unop : eunop -> fexpr -> fexpr
-| Eprim_binop : ebinop -> fexpr -> fexpr -> fexpr
-| Emux : fexpr -> fexpr -> fexpr -> fexpr
-| Evalidif : fexpr -> fexpr -> fexpr
-                                 
-.
-
-(****** Statements ******)
-Inductive ruw : Set :=
-| old | new | undefined.
-
-Record fmem : Type :=
-  mk_fmem
-    {
-      mid : var;
-      data_type : fexpr;
-      depth : nat;
-      reader : seq var;
-      writer : seq var;                    
-      read_latency : nat;
-      write_latency : nat;
-      read_under_write : ruw
-    }.
-
-Record freg : Type :=
-  mk_freg
-    {
-      rid : var;
-      type : fexpr;
-      reset : seq fexpr
-    }.
-
-Inductive fstmt : Type :=
-| Sskip
-| Swire : var -> fgtyp -> fstmt
-| Sreg : freg -> fstmt
-| Smem : fmem -> fstmt
-| Sinst : var -> var -> fstmt
-| Snode : var -> fexpr -> fstmt
-| Sfcnct : fexpr -> fexpr -> fstmt
-| Spcnct : fexpr -> fexpr -> fstmt
-| Sinvalid : var -> fstmt
-| Sattach : seq var -> fstmt
-| Swhen : fexpr -> fstmt -> fstmt -> fstmt
-| Sstop : fexpr -> fexpr -> nat -> fstmt
-| Sprintf (* TBD *)
-| Sassert (* TBD *)
-| Sassume (* TBD *)
-| Sdefname : var -> fstmt (* TBD *)
-| Sparam : var -> fexpr -> fstmt (* TBD *)
-.
-
-Inductive fport : Type :=
-| Finput : fexpr -> fport
-| Foutput : fexpr -> fport
-.
-
-(* TBD *)
-Inductive fmodule : Type :=
-| FInmod : var -> seq fport -> seq fstmt -> fmodule
-| FExmod : var -> seq fport -> seq fstmt -> fmodule
-.
-
-Definition fcircuit := var -> seq fmodule.
+  Definition fgtyp_eqMixin := EqMixin fgtyp_eqP.
+  Canonical fgtyp_eqType := Eval hnf in EqType fgtyp fgtyp_eqMixin.
 
 
+  Delimit Scope fgtyp_scope with fgtyp.
+
+  (* Integer, bitvector or ssrint, TBD *)
+
+  (* Fix-point, TBD *)
+
+  (* Analog, TBD *)
+
+  (* Vector, TBD *)
+
+
+  (****** Syntax ******)
+
+  (****** Expressions ******)
+
+  Inductive ucast : Set :=
+  | AsUInt | AsSInt | AsFixed | AsClock.
+
+  Inductive eunop : Set :=
+  | Upadding : nat -> eunop
+  | Ucast : ucast -> eunop
+  | Ushl : nat -> eunop
+  | Ushr : nat -> eunop
+  | Ucvt
+  | Uneg
+  | Unot
+  | Uandr
+  | Uorr
+  | Uxorr
+  | Uextr : nat -> nat -> eunop
+  | Uhead : nat -> eunop
+  | Utail : nat -> eunop
+  | Uincp
+  | Udecp
+  | Usetp .
+
+  Inductive bcmp : Set :=
+  | Blt | Bleq | Bgt | Bgeq | Beq | Bneq.
+
+  Inductive ebinop : Set :=
+  | Badd
+  | Bsub
+  | Bmul
+  | Bdiv
+  | Brem
+  | Bcomp: bcmp -> ebinop
+  | Bdshl
+  | Bdshr
+  | Band
+  | Bor
+  | Bxor
+  | Bcat .
+
+  (*From simplssrlib Require Import Var.*)
+  Variable var : eqType.
+
+  (* mux, valid, sub-xxx, TBD *)
+  Inductive fexpr : Type :=
+  | Econst : int -> fexpr
+  | Evar : var -> fexpr
+  | Eref : var -> fgtyp -> fexpr
+  | Efield : var -> fexpr -> fexpr
+  | Esubacc : var -> nat -> fexpr
+  | Eprim_unop : eunop -> fexpr -> fexpr
+  | Eprim_binop : ebinop -> fexpr -> fexpr -> fexpr
+  | Emux : fexpr -> fexpr -> fexpr -> fexpr
+  | Evalidif : fexpr -> fexpr -> fexpr
+                                   
+  .
+
+  (****** Statements ******)
+  Inductive ruw : Set :=
+  | old | new | undefined.
+
+  Record fmem : Type :=
+    mk_fmem
+      {
+        mid : var;
+        data_type : fexpr;
+        depth : nat;
+        reader : seq var;
+        writer : seq var;                    
+        read_latency : nat;
+        write_latency : nat;
+        read_write : ruw
+      }.
+
+  Record freg : Type :=
+    mk_freg
+      {
+        rid : var;
+        type : fexpr;
+        reset : seq fexpr
+      }.
+
+  Inductive fstmt : Type :=
+  | Sskip
+  | Swire : var -> fgtyp -> fstmt
+  | Sreg : freg -> fstmt
+  | Smem : fmem -> fstmt
+  | Sinst : var -> var -> fstmt
+  | Snode : var -> fexpr -> fstmt
+  | Sfcnct : fexpr -> fexpr -> fstmt
+  | Spcnct : fexpr -> fexpr -> fstmt
+  | Sinvalid : var -> fstmt
+  | Sattach : seq var -> fstmt
+  | Swhen : var -> fstmt -> fstmt -> fstmt
+  | Sstop : fexpr -> fexpr -> nat -> fstmt
+  | Sprintf (* TBD *)
+  | Sassert (* TBD *)
+  | Sassume (* TBD *)
+  | Sdefname : var -> fstmt (* TBD *)
+  | Sparam : var -> fexpr -> fstmt (* TBD *)
+  .
+
+  Inductive fport : Type :=
+  | Finput : fexpr -> fport
+  | Foutput : fexpr -> fport
+  .
+
+  (* TBD *)
+  Inductive fmodule : Type :=
+  | FInmod : var -> seq fport -> seq fstmt -> fmodule
+  | FExmod : var -> seq fport -> seq fstmt -> fmodule
+  .
+
+  Definition fcircuit := var -> seq fmodule.
+End RawFirrtl.
+
+
+(* A typing environment is a map from a variable to its type *)
+From simplssrlib Require Import SsrOrder FMaps.
+
+Module Type TypEnv <: SsrFMap.
+
+  Include SsrFMap.
+
+  Definition env : Type := t fgtyp.
+
+  (* The default type of a variable not in the typing environment *)
+  Parameter deftyp : fgtyp.
+
+  (* Find the type of a variable in a typing environment.
+     If a variable is not in the typing environment, return the default type. *)
+  Parameter vtyp : SE.t -> env -> fgtyp.
+
+  (* Return the size of a variable in a typing environment.
+     If a variable is not in the typing environment, return the size of the
+     default type. *)
+  Parameter vsize : SE.t -> env -> nat.
+
+  Axiom find_some_vtyp :
+    forall {x : SE.t} {ty : fgtyp} {e : env}, find x e = Some ty -> vtyp x e = ty.
+  Axiom find_none_vtyp :
+    forall {x : SE.t} {e : env}, find x e = None -> vtyp x e = deftyp.
+  Axiom vtyp_find :
+    forall {x : SE.t} {ty : fgtyp} {e : env},
+      (vtyp x e == ty) = (find x e == Some ty) || ((find x e == None) && (ty == deftyp)).
+  Axiom vtyp_add_eq :
+    forall {x y : SE.t} {ty : fgtyp} {e : env}, x == y -> vtyp x (add y ty e) = ty.
+  Axiom vtyp_add_neq :
+    forall {x y : SE.t} {ty : fgtyp} {e : env},
+      x != y -> vtyp x (add y ty e) = vtyp x e.
+  Axiom vsize_add_eq :
+    forall {x y : SE.t} {ty : fgtyp} {e : env},
+      x == y -> vsize x (add y ty e) = sizeof_fgtyp ty.
+  Axiom vsize_add_neq :
+    forall {x y : SE.t} {ty : fgtyp} {e : env},
+      x != y -> vsize x (add y ty e) = vsize x e.
+  Axiom not_mem_vtyp :
+    forall {v : SE.t} {e : env}, ~~ mem v e -> vtyp v e = deftyp.
+  Axiom vtyp_vsize :
+    forall {x : SE.t} {e : env} {ty : fgtyp},
+      vtyp x e = ty -> vsize x e = sizeof_fgtyp ty.
+
+End TypEnv.
+
+Module MakeTypEnv (V : SsrOrder) (VM : SsrFMap with Module SE := V) <:
+  TypEnv with Module SE := V.
+
+  Include VM.
+  Module Lemmas := FMapLemmas VM.
+
+  Definition env : Type := t fgtyp.
+
+  (* The default type of a variable not in the typing environment *)
+  Definition deftyp : fgtyp := Fuint 0.
+
+  (* Find the type of a variable in a typing environment.
+     If a variable is not in the typing environment, return the default type. *)
+  Definition vtyp (v : V.t) (e : env) : fgtyp :=
+    match VM.find v e with
+    | None => deftyp
+    | Some ty => ty
+    end.
+
+  (* Return the size of a variable in a typing environment.
+     If a variable is not in the typing environment, return the size of the
+     default type. *)
+  Definition vsize (v : V.t) (e : env) : nat := sizeof_fgtyp (vtyp v e).
+
+  Lemma find_some_vtyp {x ty e} : find x e = Some ty -> vtyp x e = ty.
+  Proof. move=> H. rewrite /vtyp H. reflexivity. Qed.
+
+  Lemma find_none_vtyp {x e} : find x e = None -> vtyp x e = deftyp.
+  Proof. move=> H. rewrite /vtyp H. reflexivity. Qed.
+
+  Lemma vtyp_find {x ty e} :
+    (vtyp x e == ty) = (find x e == Some ty) || ((find x e == None) && (ty == deftyp)).
+  Proof.
+    dcase (find x e); case.
+    - move=> a Hfind. rewrite (find_some_vtyp Hfind) /= orbF. case Heq: (a == ty).
+      + by rewrite (eqP Heq) eqxx.
+      + symmetry. apply/eqP => H. case: H => H. rewrite H eqxx in Heq. discriminate.
+    - move=> Hnone. rewrite (find_none_vtyp Hnone) eqxx /=. rewrite eq_sym.
+      reflexivity.
+  Qed.
+
+  Lemma vtyp_add_eq {x y ty e} : x == y -> vtyp x (add y ty e) = ty.
+  Proof. rewrite /vtyp /add => H. by rewrite (Lemmas.find_add_eq H). Qed.
+
+  Lemma vtyp_add_neq {x y ty e} : x != y -> vtyp x (add y ty e) = vtyp x e.
+  Proof.
+    move/negP=> Hxy. rewrite /vtyp /add. by rewrite (Lemmas.find_add_neq Hxy).
+  Qed.
+
+  Lemma vsize_add_eq {x y ty e} : x == y -> vsize x (add y ty e) = sizeof_fgtyp ty.
+  Proof. rewrite /vsize=> H. by rewrite (vtyp_add_eq H). Qed.
+
+  Lemma vsize_add_neq {x y ty e} : x != y -> vsize x (add y ty e) = vsize x e.
+  Proof. rewrite /vsize => H. by rewrite (vtyp_add_neq H). Qed.
+
+  Lemma not_mem_vtyp v e : ~~ mem v e -> vtyp v e = deftyp.
+  Proof. rewrite /vtyp => H. by rewrite Lemmas.not_mem_find_none. Qed.
+
+  Lemma vtyp_vsize x e ty : vtyp x e = ty -> vsize x e = sizeof_fgtyp ty.
+  Proof. rewrite /vsize /vtyp. move=> ->. reflexivity. Qed.
+
+End MakeTypEnv.
+
+
+(*Module TE <: TypEnv := MakeTypEnv VarOrder VM.*)
+(*Module SSATE <: TypEnv := MakeTypEnv SSAVarOrder SSAVM.*)
 
 (****** Semantics ******)
 
-
+(*
 Record fstate : Type :=
   mk_state
     {
       fregs : seq freg;
       fmems : seq fmem
     }.
+*)
+(* TBD *)
 
 (* TBD *)
-Parameter eval_fexpr : fstate -> fexpr -> fstate.
-
-(* TBD *)
-Parameter eval_fstmt : fstate -> fstmt -> fstate.
+(*Parameter eval_fstmt : fstate -> fstmt -> fstate.*)
